proofs/proofsystem/Tactics.v
@@ -1,0 +1,755 @@
+(*On top of the natural deduction proof system, we build a nicer
+  tactic-based version*)
+Require Export NatDed.
+From mathcomp Require Export all_ssreflect.
+Set Bullet Behavior "Strict Subproofs".
+
+(*Solve trivial goals*)
+
+Ltac prove_fmla_ty :=
+  apply /typecheck_formula_correct; reflexivity.
+
+Ltac prove_tm_ty :=
+  apply /check_tm_ty_spec; reflexivity.
+
+Definition check_formulas_typed (gamma: context) (l: list formula): bool :=
+  all (typecheck_formula gamma) l.
+
+Lemma check_formulas_typed_correct gamma l:
+  reflect (Forall (formula_typed gamma) l) (check_formulas_typed gamma l).
+Proof.
+  unfold check_formulas_typed.
+  apply forallb_ForallP. intros.
+  apply typecheck_formula_correct.
+Qed.
+
+Ltac prove_fmlas_ty :=
+  apply /check_formulas_typed_correct; reflexivity.
+
+Ltac prove_valid_context :=
+  apply /check_context_correct; reflexivity.
+
+Ltac prove_closed_tm := constructor; reflexivity.
+
+(*Intros*)
+
+(*This is basically just [D_forallI]*)
+Ltac wintros c :=
+  match goal with
+  | |- derives (?g, ?d, (Fquant Tforall ?x ?f)) =>
+    apply (D_forallI g d x f c);
+    [reflexivity | prove_fmlas_ty | prove_closed |];
+    unfold safe_sub_f; simpl
+  | |- _ => fail "wintros requires goal to be (Fquant Tforall x f)"
+  end.
+
+(*Assert*)
+Ltac wassert name f :=
+  match goal with
+  | |- derives (?g, ?d, ?goal) =>
+    apply (D_assert g d name f goal)
+  | |- _ => fail "Can only assert for a derivation"
+  end.
+
+(*Specialize*)
+(*If hypothesis H has form Fquant Tforall x f,
+  then wspecialize H t replaces H with hypothesis f[t/x]*)
+
+Definition add_hyp (delta : list (string * formula)) name f_new :=
+  (name, f_new) :: delta.
+
+Definition remove_hyp (delta: list (string * formula)) name :=
+  filter (fun x => negb (String.eqb (fst x) name)) delta.
+
+(*TODO: move*)
+(*We can permute the hypotheses*)
+Definition perm_trans (delta': list (string * formula)) : trans :=
+  fun t =>
+  if perm_eq (task_delta t) delta' then 
+  [mk_task (task_gamma t) delta' (task_goal t)] else [t].
+
+Lemma perm_trans_sound delta': sound_trans (perm_trans delta').
+Proof.
+  unfold sound_trans, perm_trans. intros.
+  destruct (perm_eq (task_delta t) delta') eqn : Hperm;
+  [| apply H; simpl; auto].
+  specialize (H _ (ltac:(left; reflexivity))).
+  destruct t as [[gamma delta] goal]; simpl_task.
+  unfold task_valid in *. destruct H as [Hwf Hval].
+  split; auto. intros. simpl_task.
+  specialize (Hval gamma_valid Hwf).
+  unfold log_conseq in *.
+  intros. specialize (Hval pd pf pf_full).
+  erewrite satisfies_irrel. apply Hval.
+  intros. erewrite satisfies_irrel. apply H.
+  Unshelve.
+  apply (perm_map snd) in Hperm.
+  apply perm_mem in Hperm.
+  apply /inP. rewrite Hperm. by apply /inP.
+Qed.
+
+Lemma Forall_perm {A: eqType} {s1 s2: seq A} {p: A -> Prop}:
+  Forall p s1 ->
+  perm_eq s1 s2 ->
+  Forall p s2.
+Proof.
+  rewrite !Forall_forall.
+  move=>Hall Hperm x /inP.
+  rewrite -(perm_mem Hperm) => /inP.
+  by apply Hall.
+Qed.
+
+Theorem D_perm gamma delta delta' goal:
+  perm_eq delta delta' ->
+  derives (gamma, delta', goal) ->
+  derives (gamma, delta, goal).
+Proof.
+  intros.
+  eapply (D_trans (perm_trans delta')); auto.
+  - inversion H0; subst. destruct H1.
+    constructor; simpl_task; auto.
+    + apply (Forall_perm task_delta_typed).
+      apply perm_map. by rewrite perm_sym.
+    + move: task_hyp_nodup => /Typechecker.uniqP Huniq. 
+      apply /Typechecker.uniqP.
+      by rewrite (perm_uniq (perm_map fst H)).
+  - apply perm_trans_sound.
+  - unfold perm_trans. simpl_task. rewrite H.
+    by intros x [<- | []].
+Qed.
+
+Definition replace_hyp (delta: list (string * formula)) (name: string)
+  (f_new: formula): list (string * formula) :=
+  map (fun x => (fst x, 
+    if String.eqb (fst x) name then f_new else snd x)) delta.
+
+Lemma perm_eq_middle {A: eqType} (s1 s2: seq A) (x: A):
+  perm_eq (x :: (s1 ++ s2)) (s1 ++ x :: s2).
+Proof.
+  by rewrite -!cat_rcons -cat_cons perm_cat2r 
+    perm_sym perm_rcons perm_refl.
+Qed. 
+
+Lemma replace_hyp_cat d1 d2 name f_new:
+  replace_hyp (d1 ++ d2) name f_new =
+  replace_hyp d1 name f_new ++ replace_hyp d2 name f_new.
+Proof.
+  by rewrite /replace_hyp map_cat.
+Qed.
+
+Lemma remove_hyp_cat d1 d2 name:
+  remove_hyp (d1 ++ d2) name =
+  remove_hyp d1 name ++ remove_hyp d2 name.
+Proof.
+  by rewrite /remove_hyp filter_cat.
+Qed.
+
+Lemma remove_hyp_notin delta name:
+  ~ In name (map fst delta) ->
+  remove_hyp delta name = delta.
+Proof.
+  move=> Hnotin. apply /all_filterP. apply /allP. 
+  move=> x /inP Hinx.
+  case: (String.eqb_spec x.1 name)=>// Heq.
+  exfalso. apply Hnotin. rewrite in_map_iff.
+  by exists x.
+Qed.
+
+Lemma replace_hyp_notin delta name f_new:
+  ~ In name (map fst delta) ->
+  replace_hyp delta name f_new = delta.
+Proof.
+  move=> Hnotin.
+  apply map_id_in. move=> x /inP Hinx.
+  case: (String.eqb_spec x.1 name) => Heq //.
+  - exfalso. apply Hnotin. rewrite in_map_iff.
+    by exists x.
+  - clear. by case: x.
+Qed.
+
+Lemma replace_hyp_perm delta name f_new :
+  NoDup (map fst delta) ->
+  In name (map fst delta) ->
+  perm_eq (replace_hyp delta name f_new)
+    ((name, f_new) :: (remove_hyp delta name)).
+Proof.
+  move=> Huniq Hin.
+  (*rewrite /replace_hyp/remove_hyp.*)
+  rewrite in_map_iff in Hin.
+  destruct Hin as [elt [Hname Hinelt]]; subst.
+  apply in_split in Hinelt.
+  destruct Hinelt as [l1 [l2 Heql]]; subst.
+  rewrite replace_hyp_cat remove_hyp_cat /= String.eqb_refl/=.
+  rewrite perm_sym.
+  (*Now need to simplify these lists because elt does not appear*)
+  move: Huniq. rewrite map_cat NoDup_app_iff /= => [[Hn1 [Hn2 [_ /( _ elt.1 ltac:(auto))]]]].
+  move=> Hnotelt. inversion Hn2; subst.
+  rewrite !remove_hyp_notin // !replace_hyp_notin //.
+  apply perm_eq_middle.
+Qed.
+
+(*TODO: replace - stronger weaken*)
+Definition weaken_trans delta' : trans :=
+  fun t =>
+  if sublistb (map snd delta') (map snd (task_delta t)) (*&&
+    uniq delta'*) then
+  [mk_task (task_gamma t) delta' (task_goal t)]
+  else [t].
+
+  (*TODO: use incl?*)
+Lemma sublist_map {A B: Type} (f: A -> B) (l1 l2: list A):
+  sublist l1 l2 ->
+  sublist (map f l1) (map f l2).
+Proof.
+  apply incl_map.
+Qed.
+
+Lemma weaken_trans_sound delta': sound_trans (weaken_trans delta').
+Proof.
+  unfold sound_trans, weaken_trans.
+  intros.
+  revert H.
+  case: (sublistb [seq i.2 | i <- delta'] [seq i.2 | i <- task_delta t]) /sublistbP => Hsub;
+  intros;[| apply H; simpl; auto].
+  specialize (H _ ltac:(left; auto)).
+  destruct t as[[gamma delta] goal]; simpl_task.
+  unfold task_valid in *. destruct H as [Hwf Hval]; split; auto; simpl_task.
+  intros.
+  specialize (Hval gamma_valid Hwf).
+  unfold log_conseq in *. intros.
+  specialize (Hval pd pf pf_full). erewrite satisfies_irrel.
+  apply Hval. intros. erewrite satisfies_irrel. apply H.
+  Unshelve.
+  revert Hd. apply Hsub.
+Qed.
+
+(*We can always add new hypotheses*)
+Theorem D_weaken gamma delta delta' goal:
+  NoDup (map fst delta) ->
+  Forall (formula_typed gamma) (map snd delta) ->
+  sublist (map snd delta') (map snd delta) ->
+  derives (gamma, delta', goal) ->
+  derives (gamma, delta, goal).
+Proof.
+  intros Hn Hsub Htys Hder.
+  eapply (D_trans (weaken_trans delta')); auto.
+  - inversion Hder; subst.
+    destruct H. constructor; auto.
+  - apply weaken_trans_sound.
+  - unfold weaken_trans. simpl_task.
+    case: (sublistb [seq i.2 | i <- delta'] [seq i.2 | i <- delta])
+    /sublistbP => Hsubl; try contradiction.
+    intros x [<- | []]; auto.
+Qed.
+
+(*Rename a hypothesis to an unused name*)
+
+Definition rename_hyp (delta: list (string * formula)) name1 name2 :
+  list (string * formula) :=
+  map (fun x => (if String.eqb (fst x) name1 then name2 else (fst x), snd x)) delta.
+
+Lemma map_snd_rename_hyp delta name1 name2:
+  List.map snd (rename_hyp delta name1 name2) = List.map snd delta.
+Proof.
+  unfold rename_hyp. rewrite map_map. reflexivity.
+Qed.
+
+
+(*Definition rename_trans name1 name2 : trans :=
+  fun t =>
+  [mk_task (task_gamma t) 
+    (rename_hyp (task_delta t) name1 name2) (task_goal t)].
+
+Lemma rename_trans_sound name1 name2: sound_trans (rename_trans name1 name2).
+Proof.
+  unfold sound_trans, rename_trans.
+  intros.
+  specialize (H _ ltac:(left; auto)).
+  destruct t as [[gamma delta] goal].
+  simpl_task.
+  unfold task_valid in *. 
+  destruct H as [Hwf Hval]. split; auto.
+  intros. simpl_task.
+  specialize (Hval gamma_valid Hwf).
+  unfold log_conseq in *. intros.
+  specialize (Hval pd pf pf_full).
+  erewrite satisfies_irrel. apply Hval.
+  intros. erewrite satisfies_irrel. apply H.
+  Unshelve.
+  rewrite map_snd_rename_hyp in Hd. auto.
+Qed.*)
+
+(*TODO: move*)
+Lemma rename_hyp_same delta n: 
+  rename_hyp delta n n = delta.
+Proof.
+  unfold rename_hyp.
+  apply map_id_in=> x /inP Hinx.
+  by case: (String.eqb_spec x.1 n)=>[ | _];
+  clear; case: x=>//= a b ->.
+Qed.
+
+Lemma rename_hyp_cat d1 d2 n1 n2:
+  rename_hyp (d1 ++ d2) n1 n2 =
+  rename_hyp d1 n1 n2 ++
+  rename_hyp d2 n1 n2.
+Proof.
+  by rewrite /rename_hyp map_cat.
+Qed.
+
+Lemma rename_hyp_notin delta n1 n2:
+  ~ In n1 (map fst delta) ->
+  rename_hyp delta n1 n2 = delta.
+Proof.
+  intros Hnotin. rewrite /rename_hyp.
+  apply map_id_in=> x /inP Hinx.
+  case: (String.eqb_spec x.1 n1) => Heq.
+  - subst. exfalso. apply Hnotin. rewrite in_map_iff.
+    by exists x.
+  - clear. by case: x.
+Qed.
+
+Lemma rename_hyp_idem delta n1 n2:
+  ~ In n2 (map fst delta) ->
+  rename_hyp (rename_hyp delta n1 n2) n2 n1 = delta.
+Proof.
+  intros Hnotin.
+  unfold rename_hyp. rewrite -map_comp/=.
+  apply map_id_in => x /inP Hinx/=.
+  case: (String.eqb_spec x.1 n1) => Hx1n; subst.
+  - rewrite String.eqb_refl; clear; by case: x.
+  - case: (String.eqb_spec x.1 n2) => Hx2n; subst.
+    + exfalso. apply Hnotin. rewrite in_map_iff. 
+      by exists x.
+    + clear; by case: x.
+Qed.
+
+Lemma rename_hyp_nodup delta n1 n2:
+  ~In n2 (map fst delta) ->
+  NoDup (map fst delta) ->
+  NoDup (map fst (rename_hyp delta n1 n2)).
+Proof.
+  intros Hnotin Hnodup.
+  destruct (in_dec string_dec n1 (map fst delta)); last by
+  rewrite rename_hyp_notin.
+  rewrite in_map_iff in i.
+  destruct i as [e [Hn1 Hine]]; subst.
+  apply in_split in Hine.
+  destruct Hine as [l1 [l2 Hdelta]]; subst.
+  revert Hnodup Hnotin.
+  rewrite rename_hyp_cat /= String.eqb_refl !map_cat/=
+  NoDup_app_iff in_app_iff /= => [[Hn1 [Hn2 [Hno1 Hnot2]]]] Hnotin.
+  not_or Hn2.
+  have Hnote1: (~ In e.1 [seq i.1 | i <- l1]). {
+    intros Hin. apply (Hnot2 e.1); auto.
+  }
+  inversion Hn2; subst.
+  rename H1 into Hnote2.
+  clear Hn2; rename H2 into Hn2.
+  rewrite NoDup_app_iff !rename_hyp_notin //.
+  split_all=>//.
+  constructor; auto.
+  - intros x Hinx1 Hinx2.
+    simpl in Hinx2. destruct Hinx2; subst; auto.
+    apply (Hnot2 x); auto.
+  - simpl. intros x [Hx | Hinx1] Hinx2; subst; auto.
+    apply (Hnot2 x); auto.
+Qed.
+
+Lemma renamed_notin delta n1 n2:
+  n1 <> n2 ->
+  ~ In n1 (map fst (rename_hyp delta n1 n2)).
+Proof.
+  intros Hneq.
+  unfold rename_hyp. rewrite -map_comp/= => Hin.
+  rewrite in_map_iff in Hin.
+  destruct Hin as [e [Hn1 Hine]]; subst.
+  simpl in Hn1.
+  destruct (String.eqb_spec e.1 n1)=>//.
+  subst. auto.
+Qed. 
+
+Lemma rename_hyp_nodup_iff delta n1 n2:
+  ~In n2 (map fst delta) ->
+  NoDup (map fst delta) <->
+  NoDup (map fst (rename_hyp delta n1 n2)).
+Proof.
+  intros Hnotin.
+  split; intros.
+  - apply rename_hyp_nodup; auto.
+  - rewrite <- (rename_hyp_idem delta n1 n2); auto.
+    apply rename_hyp_nodup; auto.
+    destruct (String.eqb_spec n1 n2).
+    {
+      subst. by rewrite rename_hyp_same.
+    }
+    by apply renamed_notin.
+Qed.
+
+Theorem D_rename gamma delta name1 name2 goal:
+  (*NoDup (map fst delta) ->*)
+  (name1 = name2 \/ ~ In name2 (map fst delta)) ->
+  derives (gamma, rename_hyp delta name1 name2, goal) ->
+  derives (gamma, delta, goal).
+Proof.
+  intros.
+  apply (D_weaken _ _ (rename_hyp delta name1 name2)); auto.
+  - inversion H0; subst.
+    destruct H1; simpl_task.
+    destruct H; subst.
+    + rewrite rename_hyp_same in task_hyp_nodup; auto.
+    + rewrite rename_hyp_nodup_iff. apply task_hyp_nodup. auto.
+  - inversion H0; subst. destruct H1; simpl_task.
+    rewrite map_snd_rename_hyp in task_delta_typed; auto.
+  - rewrite -list_map_map map_snd_rename_hyp.
+    apply sublist_refl.
+Qed.
+
+(*TDOO: autoate - make task_with_delta, single trans, etc*)
+
+(*TODO: move to GenElts*)
+Require Import GenElts.
+
+Definition gen_names (n: nat) (l: list string) : list string :=
+  gen_notin nth_str string_dec n l.
+
+Lemma gen_names_length n l:
+  List.length (gen_names n l) = n.
+Proof.
+  apply gen_notin_length. apply nth_str_inj.
+Qed.
+
+Lemma gen_names_nodup n l:
+  NoDup (gen_names n l).
+Proof.
+  apply gen_notin_nodup. apply nth_str_inj.
+Qed.
+
+Lemma gen_names_notin (n: nat) (l: list string):
+  forall x, In x (gen_names n l) -> ~ In x l.
+Proof.
+  intros. apply gen_notin_notin in H. auto.
+Qed.
+
+Definition gen_name (l: list string) : string :=
+  List.nth 0 (gen_names 1 l) EmptyString.
+
+Lemma gen_name_notin (l: list string):
+  ~ In (gen_name l) l.
+Proof.
+  unfold gen_name.
+  pose proof (gen_names_length 1 l).
+  destruct (gen_names 1 l) eqn : Heqs;
+  inversion H.
+  destruct l0; inversion H1.
+  simpl. 
+  pose proof (gen_names_notin 1 l s).
+  apply H0. rewrite Heqs; simpl; auto.
+Qed.
+
+Lemma remove_rename_sublist delta n1 n2:
+  sublist (remove_hyp delta n1) (rename_hyp delta n1 n2).
+Proof.
+  unfold sublist, remove_hyp, rename_hyp.
+  move=> x /inP.
+  rewrite mem_filter => /andP[Hneq Hinx].
+  apply /inP /mapP. exists x=>//.
+  apply negbTE in Hneq.
+  rewrite Hneq. clear. by case: x.
+Qed.
+
+(*A meta-theorem about derivations: if we can prove some
+  goal f_new, then we can replace any hypothesis with
+  this goal and prove what we originally wanted*)
+Lemma derives_replace_hyp gamma delta goal name f_new:
+  derives (gamma, delta, f_new) ->
+  derives (gamma, replace_hyp delta name f_new, goal) ->
+  derives (gamma, delta, goal).
+Proof.
+  intros.
+  assert (Hwf: task_wf (gamma, delta, f_new)). {
+    inversion H; subst; auto.
+  }
+  destruct (in_dec string_dec name (map fst delta)).
+  2: {
+    rewrite replace_hyp_notin in H0; auto.
+  }
+  (*TODO: replace D_perm with D_weaken*)
+  eapply D_perm in H0.
+  2: {
+    rewrite perm_sym.
+    apply replace_hyp_perm; auto.
+    inversion H; subst.
+    destruct H1. auto.
+  }
+  (*Need to weaken by adding old fmla, so we rename new name*)
+  (*Get a string not in the list*)
+  assert (exists s, ~ In s (map fst delta)). {
+    exists (gen_name (map fst delta)). apply gen_name_notin.
+  }
+  destruct H1 as [name2 Hnotin].
+  (*We will rename the old hyp name to name2*)
+  apply D_rename with(name1:=name)(name2:=name2); auto.
+  assert (Hneq: name <> name2). {
+    intro C; subst; contradiction.
+  }
+  apply D_assert with(name:=name)(A:=f_new).
+  - apply D_rename with (name1:=name2)(name2:=name).
+    { right. apply renamed_notin. auto. }
+    rewrite rename_hyp_idem; auto.
+  - assert (A:=H0). revert H0. apply D_weaken; auto.
+    + simpl. constructor.
+      * apply renamed_notin; auto.
+      * rewrite <- rename_hyp_nodup_iff; auto.
+        destruct Hwf. auto.
+    + simpl. rewrite <- list_map_map, map_snd_rename_hyp.
+      destruct Hwf; simpl_task.
+      destruct task_goal_typed; simpl_task.
+      constructor; auto.
+    + simpl. unfold sublist.
+      simpl.
+      intros x [Hx | Hinx]; subst; auto. right.
+      revert Hinx. apply sublist_map. apply remove_rename_sublist.
+Qed.
+
+Definition find_hyp (delta: list (string * formula)) name :=
+  get_assoc_list string_dec delta name.
+
+(*A "specialize" tactic*)
+Lemma derives_specialize gamma delta goal name (t: term) x f:
+  find_hyp delta name = Some (Fquant Tforall x f) ->
+  term_has_type gamma t (snd x) ->
+  closed_tm t ->
+  task_wf (gamma, delta, Fquant Tforall x f) ->
+  derives (gamma, replace_hyp delta name (safe_sub_f t x f), goal) ->
+  derives (gamma, delta, goal).
+Proof.
+  unfold find_hyp.
+  intros Hget Hty Hclosed Hwf.
+  apply get_assoc_list_some in Hget.
+  apply derives_replace_hyp.
+  apply D_forallE; auto.
+  apply D_axiom; simpl_task; auto.
+  rewrite in_map_iff. exists (name, Fquant Tforall x f); auto.
+Qed.
+
+(*And now the tactic*)
+
+Ltac wspecialize name tm :=
+  eapply (derives_specialize _ _ _ name tm);
+  [reflexivity | prove_tm_ty | prove_closed_tm | prove_task_wf |];
+  unfold replace_hyp; simpl;
+  unfold safe_sub_f; simpl.
+
+(*Assumption*)
+Ltac wassumption :=
+  apply D_axiom; [prove_task_wf | apply /inP; reflexivity].
+
+(*f_equal*)
+Ltac wf_equal :=
+  match goal with
+  | |- derives (?g, ?d, Feq ?ty (Tfun ?f ?tys ?tms1) (Tfun ?f ?tys ?tms2)) =>
+    apply (D_f_equal g d f tys tms1 tms2 ty);
+    [reflexivity | reflexivity | prove_tm_ty | prove_tm_ty |
+      reflexivity |];
+    simpl; repeat constructor
+  | _ => fail "f_equal requires goal in form derives (gamma, delta, f xn = f yn)"
+  end.
+
+(*reflexivity*)
+Ltac wreflexivity :=
+  match goal with
+  | |- derives (?g, ?d, Feq ?ty ?t ?t) =>
+      apply (D_eq_refl g d ty t);
+      [prove_valid_context | prove_fmlas_ty |
+      apply /Typechecker.uniqP; reflexivity |
+      prove_closed_tm | prove_tm_ty ]
+  | _ => fail "reflexivity requires goal of form (x = x)"
+  end.
+
+(*Rewrite*)
+Lemma derives_rewrite gamma delta goal name t1 t2 ty:
+  find_hyp delta name = Some (Feq ty t1 t2) ->
+  Logic.closed gamma goal ->
+  Logic.closed gamma (Feq ty t1 t2) ->
+  derives (gamma, delta, replace_tm_f t1 t2 goal) ->
+  derives (gamma, delta, goal).
+Proof.
+  unfold find_hyp; intros Hget Hclosed Hc2 Hd.
+  apply get_assoc_list_some in Hget.
+  apply (D_rewrite _ _ t1 t2 ty); auto.
+  apply D_axiom; simpl_task. 
+  - inversion Hd; subst. destruct H; subst; constructor;
+    auto.
+  - rewrite in_map_iff. exists (name, Feq ty t1 t2); auto.
+Qed.
+
+Ltac wrewrite H :=
+  match goal with
+  | |- derives (?g, ?d, ?f) =>
+    eapply (derives_rewrite g d f H);
+    [reflexivity | prove_closed | prove_closed |];
+    unfold replace_tm_f; simpl
+  | _ => fail "Usage: rewrite H, where H : t1 = t2"
+  end.
+
+(*Symmetry*)
+Ltac wsymmetry := apply D_eq_sym.
+
+(*TODO: move*)
+Lemma map_fst_replace_hyp delta name f_new:
+  List.map fst (replace_hyp delta name f_new) = List.map fst delta.
+Proof.
+  unfold replace_hyp. rewrite map_map. reflexivity.
+Qed.
+
+(*Lemma replace_hyp_snd {P: formula -> Prop} delta name f:
+  NoDup (map fst delta) ->
+  Forall P (List.map snd (replace_hyp delta name f)) ->
+  P f ->
+  Forall P (List.map snd delta).
+Proof.
+  intros Hn Hall Hf.
+  destruct (in_dec string_dec name (map fst delta)).
+  2: {
+    rewrite replace_hyp_notin in Hall; auto.
+  }
+  (*
+  rewrite in_map_iff in i.
+  destruct i as [e [Hname Hine]]; subst.
+  apply in_split in Hine.
+  destruct Hine as [l1 [l2 Hdelta]]; subst.
+  revert Hall.
+  rewrite replace_hyp_cat; simpl;
+  rewrite !map_app; simpl.
+  rewrite String.eqb_refl.
+  rewrite !replace_hyp_notin. simpl.
+  rewrite replace_hyp_cat in Hall.
+  rewrite map_cat in Hall.*)
+  eapply Forall_perm in Hall.
+  2: apply perm_map; apply replace_hyp_perm.
+  all: auto.
+  revert Hall. rewrite !Forall_forall; intros.
+  simpl in Hall. rewrite in_map_iff in H.
+  destruct H as [e [Hx Hine]]; subst.
+  rewrite in_map_iff in i.
+  destruct i as [e2 [Hname Hine2]]; subst.
+  destruct (String.eqb_spec e.1 e2.1).
+  - apply Hall. left.
+    eapply nodup_fst_inj.
+    apply Hn. apply Hin
+  
+  Search NoDup List.map fst.
+  unfold remove_hyp in Hall.
+  specialize (Hall e.2).
+
+  2: apply perm_eq_map.
+  Search replace_hyp perm_eq.
+  Search Forall perm_eq.
+  unfold replace_hyp in Hall.
+
+*)
+
+(*rewrite in*)
+Lemma derives_rewrite_in gamma delta goal name1 name2 ty t1 t2 f:
+  find_hyp delta name1 = Some (Feq ty t1 t2) ->
+  find_hyp delta name2 = Some f ->
+  Logic.closed gamma (replace_tm_f t1 t2 f) ->
+  Logic.closed gamma (Feq ty t1 t2) ->
+  Logic.closed gamma f ->
+  Forall (formula_typed gamma) (List.map snd delta) ->
+  derives (gamma, replace_hyp delta name2 (replace_tm_f t1 t2 f), goal) ->
+  derives (gamma, delta, goal).
+Proof.
+  intros Hf1 Hf2 Hc1 Hc2 Hc3 Hty Hd.
+  assert (A:=Hd). revert A.
+  apply derives_replace_hyp.
+  apply get_assoc_list_some in Hf1, Hf2.
+  eapply D_rewrite2 with(ty:=ty); auto;
+  apply D_axiom; simpl_task.
+  - inversion Hd; subst.
+    destruct H; subst.
+    constructor; auto; simpl_task.
+    rewrite map_fst_replace_hyp in task_hyp_nodup. auto.
+  - rewrite in_map_iff. exists (name1, Feq ty t1 t2); auto.
+  - inversion Hd; subst.
+    inversion H; subst.
+    constructor; auto; simpl_task.
+    rewrite map_fst_replace_hyp in task_hyp_nodup. auto.
+  - rewrite in_map_iff. exists (name2, f). auto.
+Qed.
+
+(*Usage: rewrite_in H1 H2: H1 : t1 = t2, rewrite this in H2*)
+Ltac wrewrite_in H1 H2 :=
+  eapply derives_rewrite_in with(name1:=H1)(name2:=H2);
+  [reflexivity | reflexivity | prove_closed | prove_closed
+    | prove_closed | prove_fmlas_ty |];
+  unfold replace_tm_f; simpl.
+
+(*Symmetry in*)
+Lemma derives_symmetry_in gamma delta goal name t1 t2 ty:
+  find_hyp delta name = Some (Feq ty t1 t2) ->
+  Logic.closed gamma (Feq ty t1 t2) ->
+  Forall (formula_typed gamma) (List.map snd delta) ->
+  derives (gamma, replace_hyp delta name (Feq ty t2 t1), goal) ->
+  derives (gamma, delta, goal).
+Proof.
+  intros Hf Hclosed Hall Hd. apply get_assoc_list_some in Hf.
+  assert (A:=Hd).
+  revert A. apply derives_replace_hyp.
+  apply D_eq_sym. apply D_axiom.
+  - inversion Hd; subst. destruct H; subst;
+    constructor; auto; simpl_task.
+    rewrite map_fst_replace_hyp in task_hyp_nodup. auto.
+  - rewrite in_map_iff. exists (name, Feq ty t1 t2); auto.
+Qed.
+
+Ltac wsymmetry_in H :=
+  eapply (derives_symmetry_in) with (name:=H);
+  [reflexivity | prove_closed | prove_fmlas_ty |];
+  unfold replace_hyp; simpl.
+
+(*TODO: maybe add custom simpl tactic after all of these?*)
+
+(*Apply (only for hypotheses)*)
+
+(*Note: right now, this only works for 1 hypothesis. Should make
+  a version for arbitrary (by converting to P1 /\ ... /\ Pn -> H)*)
+Lemma derives_apply gamma delta goal name f:
+  find_hyp delta name = Some (Fbinop Timplies f goal) ->
+  Logic.closed gamma goal ->
+  derives (gamma, delta, f) ->
+  derives (gamma, delta, goal).
+Proof.
+  intros Hf Hc Hd.
+  apply get_assoc_list_some in Hf.
+  apply (D_implE _ _ f goal); auto.
+  apply D_axiom.
+  - inversion Hd; subst. destruct H; subst.
+    constructor; auto; simpl_task.
+    apply closed_binop; auto.
+  - rewrite in_map_iff. exists (name, Fbinop Timplies f goal); auto.
+Qed.
+
+Ltac wapply H :=
+  eapply (derives_apply) with(name:=H);
+  [reflexivity | prove_closed |].
+
+
+(*TODO: apply (for impl), apply in*)
+
+
+(*Specialize _ as _*)
+
+
+
+  (*Theorem D_forallI gamma delta x f c:
+  (*c is not used*)
+  negb (in_bool string_dec c (map (fun (x: funsym) => s_name x) 
+    (sig_f gamma))) ->
+  (*delta and f are typed under gamma (they do not use the new symbol)*)
+  Forall (formula_typed gamma) (map snd delta) ->
+  closed gamma (Fquant Tforall x f) ->
+  derives (abs_fun (constsym c (snd x)) :: gamma, delta, 
+    safe_sub_f (t_constsym c (snd x)) x f) ->
+  derives (gamma, delta, Fquant Tforall x f).*)
